ironfleet/src/Dafny/Distributed/Protocol/ZooKeeper/PerformamceProof/BuggyZKInvariants.dfy
@@ -125,9 +125,12 @@ predicate Leader_Only_Send_SyncSnap(tls:TLS_State)
     requires ZK_Config_Invariant(tls.config, tls)
     requires |tls.initialZkdbState| == |tls.config|
 {
+    var target_db := tls.initialZkdbState[0];
     var l := tls.t_servers[tls.config[0]].v.leader;
     forall h | h in l.handlers ::
-        forall p | p in l.handlers[h].queuedPackets :: p.SyncSNAP?
+        forall p | p in l.handlers[h].queuedPackets :: 
+            && p.SyncSNAP?
+            && p.leaderDb == target_db
 }
 
 
@@ -174,25 +177,6 @@ lemma theorem_ZK_Buggy_Guarantee_Induction(config:Config, tls:TLS_State, tls':TL
     var targDb := tls.initialZkdbState[0];
     
     assert Starting_Leader_Does_Not_Modify_Db(tls');
-
-    forall pkt | pkt in tls'.t_environment.sentPackets
-    ensures pkt.msg.v.SyncSNAP? ==> pkt.msg.v.leaderDb == targDb
-    {
-        if pkt !in tls.t_environment.sentPackets {
-            var actor, tios:seq<TZKIo> :| actor in tls.t_servers && TLS_NextOneServer(tls, tls', actor, tios);
-            var ios := UntagLIoOpSeq(tios);
-            if actor == config[0] {
-                assert LeaderStartStep(l, l', ios);
-                assert pkt.msg.v.SyncSNAP? ==> pkt.msg.v.leaderDb == targDb;
-            } else {
-                assert tls.t_servers[actor].v.FollowerPeer?;
-                assert pkt.msg.v.SyncSNAP? ==> pkt.msg.v.leaderDb == targDb;
-            }
-        } else {
-            assert pkt.msg.v.SyncSNAP? ==> pkt.msg.v.leaderDb == targDb;
-        }
-    }
-
     assert All_Snap_Messages_Have_Same_Db(tls');
     assert Dbs_Are_Identical(tls');
     assert All_Messages_Have_Same_Zxid(tls');
